misc modernizations

thys/Efficient-Mergesort/Efficient_Sort.thy
@@ -1,9 +1,9 @@
-(*  Author:      Christian Sternagel
-    Maintainer:  Christian Sternagel
+(*  Author:      Christian Sternagel <c.sternagel@gmail.com>
+    Maintainer:  Christian Sternagel <c.sternagel@gmail.com>
 *)
 
 theory Efficient_Sort
-imports "HOL-Library.Multiset"
+  imports "HOL-Library.Multiset"
 begin
 
 text \<open>
@@ -18,35 +18,31 @@ Make sure that some binary predicate @{text P} is satisfied between
 every two consecutive elements of a list. We call such a list a
 \emph{chain} in the following.
 \<close>
-inductive
-  linked :: "('a \<Rightarrow> 'a \<Rightarrow> bool) \<Rightarrow> 'a list \<Rightarrow> bool"
-  for P::"'a \<Rightarrow> 'a \<Rightarrow> bool"
-where
-  Nil[iff]: "linked P []"
-| singleton[iff]: "linked P [x]"
-| many: "P x y \<Longrightarrow> linked P (y#ys) \<Longrightarrow> linked P (x#y#ys)"
+inductive linked for P :: "'a \<Rightarrow> 'a \<Rightarrow> bool"
+  where
+    Nil [iff]: "linked P []"
+  | singleton [iff]: "linked P [x]"
+  | many: "P x y \<Longrightarrow> linked P (y # ys) \<Longrightarrow> linked P (x # y # ys)"
 
-declare eqTrueI[OF Nil, code] eqTrueI[OF singleton, code]
+declare eqTrueI [OF Nil, code] eqTrueI [OF singleton, code]
 
-lemma linked_many_eq[simp, code]:
-  "linked P (x#y#zs) \<longleftrightarrow> P x y \<and> linked P (y#zs)"
+lemma linked_many_eq [simp, code]:
+  "linked P (x # y # zs) \<longleftrightarrow> P x y \<and> linked P (y # zs)"
   by (blast intro: linked.many elim: linked.cases)
 
 text \<open>Take the longest prefix of a list that forms a chain.\<close>
-fun take_chain :: "'a \<Rightarrow> ('a \<Rightarrow> 'a \<Rightarrow> bool) \<Rightarrow> 'a list \<Rightarrow> 'a list" where
-  "take_chain a P [] = []"
-| "take_chain a P (x#xs) = (if P a x
-    then x # take_chain x P xs
-    else [])"
+fun take_chain :: "'a \<Rightarrow> ('a \<Rightarrow> 'a \<Rightarrow> bool) \<Rightarrow> 'a list \<Rightarrow> 'a list"
+  where
+    "take_chain a P [] = []"
+  | "take_chain a P (x # xs) = (if P a x then x # take_chain x P xs else [])"
 
 text \<open>Drop the longest prefix of a list that forms a chain.\<close>
-fun drop_chain :: "'a \<Rightarrow> ('a \<Rightarrow> 'a \<Rightarrow> bool) \<Rightarrow> 'a list \<Rightarrow> 'a list" where
-  "drop_chain a P [] = []"
-| "drop_chain a P (x#xs) = (if P a x
-    then drop_chain x P xs
-    else x#xs)"
+fun drop_chain :: "'a \<Rightarrow> ('a \<Rightarrow> 'a \<Rightarrow> bool) \<Rightarrow> 'a list \<Rightarrow> 'a list"
+  where
+    "drop_chain a P [] = []"
+  | "drop_chain a P (x # xs) = (if P a x then drop_chain x P xs else x # xs)"
 
-lemma take_chain_drop_chain_id[simp]:
+lemma take_chain_drop_chain_id [simp]:
   "take_chain a P xs @ drop_chain a P xs = xs"
   by (induct xs arbitrary: a) simp_all
 
@@ -55,7 +51,7 @@ lemma linked_take_chain:
   by (induct xs arbitrary: x) simp_all
 
 lemma linked_rev_take_chain_append:
-  "linked P (x#ys) \<Longrightarrow> linked P (rev (take_chain x (\<lambda>x y. P y x) xs) @ x#ys)"
+  "linked P (x # ys) \<Longrightarrow> linked P (rev (take_chain x (\<lambda>x y. P y x) xs) @ x # ys)"
   by (induct xs arbitrary: x ys) simp_all
 
 lemma linked_rev_take_chain:
@@ -63,45 +59,46 @@ lemma linked_rev_take_chain:
   using linked_rev_take_chain_append[of P x "[]" xs] by simp
 
 lemma linked_append:
-  "linked P (xs@ys) \<longleftrightarrow> linked P xs \<and> linked P ys
-    \<and> (if xs \<noteq> [] \<and> ys \<noteq> [] then P (last xs) (hd ys) else True)"
-    (is "?lhs = ?rhs")
+  "linked P (xs @ ys) \<longleftrightarrow>
+    linked P xs \<and> linked P ys \<and>
+    (if xs \<noteq> [] \<and> ys \<noteq> [] then P (last xs) (hd ys) else True)"
+  (is "?lhs = ?rhs")
 proof
-  assume "?lhs" thus "?rhs"
+  assume "?lhs" then show "?rhs"
   proof (induct xs)
-    case (Cons x xs) thus ?case by (cases xs, simp_all) (cases ys, auto)
+    case (Cons x xs) then show ?case by (cases xs, simp_all) (cases ys, auto)
   qed simp
 next
-  assume "?rhs" thus "?lhs"
+  assume "?rhs" then show "?lhs"
   proof (induct xs)
-    case (Cons x xs) thus ?case by (cases ys, auto) (cases xs, auto)
+    case (Cons x xs) then show ?case by (cases ys, auto) (cases xs, auto)
   qed simp
 qed
 
-lemma length_drop_chain[termination_simp]:
+lemma length_drop_chain [termination_simp]:
   "length (drop_chain b P xs) \<le> length xs" (is "?P b xs")
 proof (induct xs arbitrary: b rule: length_induct)
-  fix xs::"'a list" and b
+  fix xs :: "'a list" and b
   assume IH: "\<forall>ys. length ys < length xs \<longrightarrow> (\<forall>x. ?P x ys)"
   show "?P b xs"
   proof (cases xs)
-    case (Cons y ys) with IH[rule_format, of ys y] show ?thesis by simp
+    case (Cons y ys) with IH [rule_format, of ys y] show ?thesis by simp
   qed simp
 qed
 
-lemma take_chain_map[simp]:
+lemma take_chain_map [simp]:
   "take_chain (f x) P (map f xs) = map f (take_chain x (\<lambda>x y. P (f x) (f y)) xs)"
   by (induct xs arbitrary: x) simp_all
 
 
 subsection \<open>Sorted is a Special Case of Linked\<close>
 
-lemma (in linorder) linked_le_sorted_conv[simp]:
+lemma (in linorder) linked_le_sorted_conv [simp]:
   "linked (\<le>) xs = sorted xs"
 proof
-  assume "sorted xs" thus "linked (\<le>) xs"
+  assume "sorted xs" then show "linked (\<le>) xs"
   proof (induct xs)
-    case (Cons x xs) thus ?case by (cases xs) simp_all
+    case (Cons x xs) then show ?case by (cases xs) simp_all
   qed simp
 qed (induct xs rule: linked.induct, auto)
 
@@ -109,33 +106,37 @@ lemma (in linorder) linked_less_imp_sorted:
   "linked (<) xs \<Longrightarrow> sorted xs"
   by (induct xs rule: linked.induct) auto
 
-abbreviation (in linorder) (input) lt :: "('b \<Rightarrow> 'a) \<Rightarrow> 'b \<Rightarrow> 'b \<Rightarrow> bool" where
-  "lt key x y \<equiv> key x < key y"
+abbreviation (in linorder) (input) lt :: "('b \<Rightarrow> 'a) \<Rightarrow> 'b \<Rightarrow> 'b \<Rightarrow> bool"
+  where
+    "lt key x y \<equiv> key x < key y"
 
-abbreviation (in linorder) (input) le :: "('b \<Rightarrow> 'a) \<Rightarrow> 'b \<Rightarrow> 'b \<Rightarrow> bool" where
-  "le key x y \<equiv> key x \<le> key y"
+abbreviation (in linorder) (input) le :: "('b \<Rightarrow> 'a) \<Rightarrow> 'b \<Rightarrow> 'b \<Rightarrow> bool"
+  where
+    "le key x y \<equiv> key x \<le> key y"
 
-abbreviation (in linorder) (input) gt :: "('b \<Rightarrow> 'a) \<Rightarrow> 'b \<Rightarrow> 'b \<Rightarrow> bool" where
-  "gt key x y \<equiv> key x > key y"
+abbreviation (in linorder) (input) gt :: "('b \<Rightarrow> 'a) \<Rightarrow> 'b \<Rightarrow> 'b \<Rightarrow> bool"
+  where
+    "gt key x y \<equiv> key x > key y"
 
-abbreviation (in linorder) (input) ge :: "('b \<Rightarrow> 'a) \<Rightarrow> 'b \<Rightarrow> 'b \<Rightarrow> bool" where
-  "ge key x y \<equiv> key x \<ge> key y"
+abbreviation (in linorder) (input) ge :: "('b \<Rightarrow> 'a) \<Rightarrow> 'b \<Rightarrow> 'b \<Rightarrow> bool"
+  where
+    "ge key x y \<equiv> key x \<ge> key y"
 
-lemma (in linorder) sorted_take_chain_le[simp]:
+lemma (in linorder) sorted_take_chain_le [simp]:
   "sorted (key x # map key (take_chain x (le key) xs))"
   using linked_take_chain[of "(\<le>)", of "key x" "map key xs"] by simp
 
 lemma (in linorder) sorted_rev_take_chain_gt_append:
   assumes "linked (<) (key x # map key ys)"
   shows "sorted (map key (rev (take_chain x (gt key) xs)) @ key x # map key ys)"
-  using linked_less_imp_sorted[OF linked_rev_take_chain_append[OF assms, of "map key xs"]]
+  using linked_less_imp_sorted [OF linked_rev_take_chain_append [OF assms, of "map key xs"]]
     by (simp add: rev_map)
 
-lemma mset_take_chain_drop_chain[simp]:
+lemma mset_take_chain_drop_chain [simp]:
   "mset (take_chain x P xs) + mset (drop_chain x P xs) = mset xs"
   by (induct xs arbitrary: x) (simp_all add: ac_simps)
 
-lemma mset_drop_chain_take_chain[simp]:
+lemma mset_drop_chain_take_chain [simp]:
   "mset (drop_chain x P xs) + mset (take_chain x P xs) = mset xs"
   by (induct xs arbitrary: x) (simp_all add: ac_simps)
 
@@ -160,75 +161,78 @@ sorted lists.
 fun sequences :: "('b \<Rightarrow> 'a) \<Rightarrow> 'b list \<Rightarrow> 'b list list"
   and asc :: "('b \<Rightarrow> 'a) \<Rightarrow> 'b \<Rightarrow> ('b list \<Rightarrow> 'b list) \<Rightarrow> 'b list \<Rightarrow> 'b list list"
   and desc :: "('b \<Rightarrow> 'a) \<Rightarrow> 'b \<Rightarrow> 'b list \<Rightarrow> 'b list \<Rightarrow> 'b list list"
-where
-  "sequences key (a#b#xs) =
-    (if key a > key b then desc key b [a] xs else asc key b ((#) a) xs)"
-| "sequences key xs = [xs]"
-| "asc key a f (b#bs) = (if \<not> key a > key b
-    then asc key b (f \<circ> (#) a) bs
-    else f [a] # sequences key (b#bs))"
-| "asc key a f bs = f [a] # sequences key bs"
-| "desc key a as (b#bs) = (if key a > key b
-    then desc key b (a#as) bs
-    else (a#as) # sequences key (b#bs))"
-| "desc key a as bs = (a#as) # sequences key bs"
+  where
+    "sequences key (a#b#xs) =
+      (if key a > key b then desc key b [a] xs else asc key b ((#) a) xs)"
+  | "sequences key xs = [xs]"
+  | "asc key a f (b#bs) =
+      (if \<not> key a > key b then asc key b (f \<circ> (#) a) bs
+      else f [a] # sequences key (b#bs))"
+  | "asc key a f bs = f [a] # sequences key bs"
+  | "desc key a as (b#bs) =
+      (if key a > key b then desc key b (a#as) bs
+      else (a#as) # sequences key (b#bs))"
+  | "desc key a as bs = (a#as) # sequences key bs"
 
-fun merge :: "('b \<Rightarrow> 'a) \<Rightarrow> 'b list \<Rightarrow> 'b list \<Rightarrow> 'b list" where
-  "merge key (a#as) (b#bs) = (if key a > key b
-    then b # merge key (a#as) bs
-    else a # merge key as (b#bs))"
-| "merge key [] bs = bs"
-| "merge key as [] = as"
+fun merge :: "('b \<Rightarrow> 'a) \<Rightarrow> 'b list \<Rightarrow> 'b list \<Rightarrow> 'b list"
+  where
+    "merge key (a#as) (b#bs) =
+      (if key a > key b then b # merge key (a#as) bs
+      else a # merge key as (b#bs))"
+  | "merge key [] bs = bs"
+  | "merge key as [] = as"
 
-fun merge_pairs :: "('b \<Rightarrow> 'a) \<Rightarrow> 'b list list \<Rightarrow> 'b list list" where
-  "merge_pairs key (a#b#xs) = merge key a b # merge_pairs key xs"
-| "merge_pairs key xs = xs"
+fun merge_pairs :: "('b \<Rightarrow> 'a) \<Rightarrow> 'b list list \<Rightarrow> 'b list list"
+  where
+    "merge_pairs key (a#b#xs) = merge key a b # merge_pairs key xs"
+  | "merge_pairs key xs = xs"
 
-lemma merge_Nil2[simp]: "merge key as [] = as" by (cases as) simp_all
+lemma merge_Nil2 [simp]: "merge key as [] = as" by (cases as) simp_all
 
-lemma length_merge[simp]:
+lemma length_merge [simp]:
   "length (merge key xs ys) = length xs + length ys"
   by (induct xs ys rule: merge.induct) simp_all
 
-lemma merge_pairs_length[termination_simp]:
+lemma merge_pairs_length [termination_simp]:
   "length (merge_pairs key xs) \<le> length xs"
   by (induct xs rule: merge_pairs.induct) simp_all
 
-fun merge_all :: "('b \<Rightarrow> 'a) \<Rightarrow> 'b list list \<Rightarrow> 'b list" where
-  "merge_all key [] = []"
-| "merge_all key [x] = x"
-| "merge_all key xs = merge_all key (merge_pairs key xs)"
+fun merge_all :: "('b \<Rightarrow> 'a) \<Rightarrow> 'b list list \<Rightarrow> 'b list"
+  where
+    "merge_all key [] = []"
+  | "merge_all key [x] = x"
+  | "merge_all key xs = merge_all key (merge_pairs key xs)"
 
-lemma mset_merge[simp]:
+lemma mset_merge [simp]:
   "mset (merge key xs ys) = mset xs + mset ys"
   by (induct xs ys rule: merge.induct) (simp_all add: ac_simps)
 
-lemma set_merge[simp]:
+lemma set_merge [simp]:
   "set (merge key xs ys) = set xs \<union> set ys"
-  unfolding set_mset_mset[symmetric] by simp
+  by (simp flip: set_mset_mset)
 
-lemma mset_concat_merge_pairs[simp]:
+lemma mset_concat_merge_pairs [simp]:
   "mset (concat (merge_pairs key xs)) = mset (concat xs)"
   by (induct xs rule: merge_pairs.induct) (auto simp: ac_simps)
 
-lemma set_concat_merge_pairs[simp]:
+lemma set_concat_merge_pairs [simp]:
   "set (concat (merge_pairs key xs)) = set (concat xs)"
-  unfolding set_mset_mset[symmetric] by simp
+  by (simp flip: set_mset_mset)
 
-lemma mset_merge_all[simp]:
+lemma mset_merge_all [simp]:
   "mset (merge_all key xs) = mset (concat xs)"
   by (induct xs rule: merge_all.induct) (simp_all add: ac_simps)
 
-lemma set_merge_all[simp]:
+lemma set_merge_all [simp]:
   "set (merge_all key xs) = set (concat xs)"
-  unfolding set_mset_mset[symmetric] by simp
+  by (simp flip: set_mset_mset)
 
-lemma sorted_merge[simp]:
+lemma sorted_merge [simp]:
   assumes "sorted (map key xs)" and "sorted (map key ys)"
   shows "sorted (map key (merge key xs ys))"
   using assms by (induct xs ys rule: merge.induct) (auto)
 
-lemma sorted_merge_pairs[simp]:
+lemma sorted_merge_pairs [simp]:
   assumes "\<forall>x\<in>set xs. sorted (map key x)"
   shows "\<forall>x\<in>set (merge_pairs key xs). sorted (map key x)"
   using assms by (induct xs rule: merge_pairs.induct) simp_all
@@ -238,17 +242,17 @@ lemma sorted_merge_all:
   shows "sorted (map key (merge_all key xs))"
   using assms by (induct xs rule: merge_all.induct) simp_all
 
-lemma desc_take_chain_drop_chain_conv[simp]:
-  "desc key a bs xs
-    = (rev (take_chain a (gt key) xs) @ a # bs) # sequences key (drop_chain a (gt key) xs)"
+lemma desc_take_chain_drop_chain_conv [simp]:
+  "desc key a bs xs =
+    (rev (take_chain a (gt key) xs) @ a # bs) # sequences key (drop_chain a (gt key) xs)"
 proof (induct xs arbitrary: a bs)
-  case (Cons x xs) thus ?case by (cases "key a < key x") simp_all
+  case (Cons x xs) then show ?case by (cases "key a < key x") simp_all
 qed simp
 
 lemma asc_take_chain_drop_chain_conv_append:
-  assumes "\<And>xs ys. f (xs@ys) = f xs @ ys"
-  shows "asc key a (f \<circ> (@) as) xs
-    = (f as @ a # take_chain a (le key) xs) # sequences key (drop_chain a (le key) xs)"
+  assumes "\<And>xs ys. f (xs @ ys) = f xs @ ys"
+  shows "asc key a (f \<circ> (@) as) xs =
+    (f as @ a # take_chain a (le key) xs) # sequences key (drop_chain a (le key) xs)"
 using assms
 proof (induct xs arbitrary: as a)
   case (Cons x xs)
@@ -257,22 +261,22 @@ proof (induct xs arbitrary: as a)
     case False with Cons show ?thesis by auto
   next
     case True
-    with Cons(1)[of "x" "as@[a]"] and Cons(2)
+    with Cons(1) [of "x" "as @ [a]"] and Cons(2)
       show ?thesis by (simp add: o_def)
   qed
 qed simp
 
-lemma asc_take_chain_drop_chain_conv[simp]:
-  "asc key b ((#) a) xs
-    = (a # b # take_chain b (le key) xs) # sequences key (drop_chain b (le key) xs)"
+lemma asc_take_chain_drop_chain_conv [simp]:
+  "asc key b ((#) a) xs =
+    (a # b # take_chain b (le key) xs) # sequences key (drop_chain b (le key) xs)"
 proof -
   let ?f = "(#) a"
-  have "\<And>xs ys. ((#) a) (xs@ys) = ((#) a) xs @ ys" by simp
-  from asc_take_chain_drop_chain_conv_append[of ?f key b "[]" xs, OF this]
-    show ?thesis by (simp add: o_def)
+  have "\<And>xs ys. ((#) a) (xs @ ys) = ((#) a) xs @ ys" by simp
+  from asc_take_chain_drop_chain_conv_append [of ?f key b "[]" xs, OF this]
+  show ?thesis by (simp add: o_def)
 qed
 
-lemma sequences_induct[case_names Nil singleton many]:
+lemma sequences_induct [case_names Nil singleton many]:
   assumes "\<And>key. P key []" and "\<And>key x. P key [x]"
     and "\<And>key a b xs.
     (le key a b \<Longrightarrow> P key (drop_chain b (le key) xs))
@@ -285,50 +289,49 @@ lemma sorted_sequences:
   "\<forall>x\<in>set (sequences key xs). sorted (map key x)"
 proof (induct key xs rule: sequences_induct)
   case (many key a b xs)
-  thus ?case using sorted_rev_take_chain_gt_append[of key b "[a]" xs]
+  then show ?case using sorted_rev_take_chain_gt_append [of key b "[a]" xs]
     by (cases "le key a b") (auto simp del: sorted.simps(2) simp add: sorted2_simps)
 qed simp_all
 
-lemma mset_sequences[simp]:
+lemma mset_sequences [simp]:
   "mset (concat (sequences key xs)) = mset xs"
   by (induct key xs rule: sequences_induct) (simp_all add: ac_simps)
 
-lemma filter_by_key_drop_chain_gt[simp]:
+lemma filter_by_key_drop_chain_gt [simp]:
   assumes "key b \<le> key a"
   shows "[y\<leftarrow>drop_chain b (gt key) xs. key a = key y] = [y\<leftarrow>xs. key a = key y]"
   using assms by (induct xs arbitrary: b) auto
 
-lemma filter_by_key_take_chain_gt[simp]:
+lemma filter_by_key_take_chain_gt [simp]:
   assumes "key b \<le> key a"
   shows "[y\<leftarrow>take_chain b (gt key) xs. key a = key y] = []"
   using assms by (induct xs arbitrary: b) auto
 
-lemma filter_take_chain_drop_chain[simp]:
+lemma filter_take_chain_drop_chain [simp]:
   "filter P (take_chain x Q xs) @ filter P (drop_chain x Q xs) = filter P xs"
   by (simp add: filter_append[symmetric])
 
-lemma filter_by_key_rev_take_chain_gt_conv[simp]:
-  "[y\<leftarrow>rev (take_chain b (gt key) xs). key x = key y]
-    = [y\<leftarrow>take_chain b (gt key) xs. key x = key y]"
+lemma filter_by_key_rev_take_chain_gt_conv [simp]:
+  "[y\<leftarrow>rev (take_chain b (gt key) xs). key x = key y] =
+    [y\<leftarrow>take_chain b (gt key) xs. key x = key y]"
   by (induct xs arbitrary: b) auto
 
-lemma filter_by_key_sequences[simp]:
-  "[y\<leftarrow>concat (sequences key xs). key x = key y]
-    = [y\<leftarrow>xs. key x = key y]" (is ?P)
+lemma filter_by_key_sequences [simp]:
+  "[y\<leftarrow>concat (sequences key xs). key x = key y] = [y\<leftarrow>xs. key x = key y]"
   by (induct key xs rule: sequences_induct) auto
 
-lemma merge_simp[simp]:
+lemma merge_simp [simp]:
   assumes "sorted (map key xs)"
-  shows "merge key xs (y#ys)
-    = takeWhile (ge key y) xs @ y # merge key (dropWhile (ge key y) xs) ys"
+  shows "merge key xs (y # ys) =
+    takeWhile (ge key y) xs @ y # merge key (dropWhile (ge key y) xs) ys"
   using assms by (induct xs arbitrary: y ys) (auto)
 
-lemma sorted_map_dropWhile[simp]:
+lemma sorted_map_dropWhile [simp]:
   assumes "sorted (map key xs)"
   shows "sorted (map key (dropWhile (ge key y) xs))"
-  using sorted_dropWhile[OF assms] by (simp add: dropWhile_map o_def)
+  using sorted_dropWhile [OF assms] by (simp add: dropWhile_map o_def)
 
-lemma sorted_merge_induct[consumes 1, case_names Nil IH]:
+lemma sorted_merge_induct [consumes 1, case_names Nil IH]:
   assumes "sorted (map key xs)"
     and "\<And>xs. P xs []"
     and "\<And>xs y ys. sorted (map key xs) \<Longrightarrow> P (dropWhile (ge key y) xs) ys
@@ -337,94 +340,90 @@ lemma sorted_merge_induct[consumes 1, case_names Nil IH]:
   using assms(2-) assms(1)
   by (induction_schema) (case_tac ys, simp_all, lexicographic_order)
  
-lemma filter_by_key_dropWhile[simp]:
+lemma filter_by_key_dropWhile [simp]:
   assumes "sorted (map key xs)"
   shows "[y\<leftarrow>dropWhile (\<lambda>x. key x \<le> key z) xs. key z = key y] = []"
     (is "[y\<leftarrow>dropWhile ?P xs. key z = key y] = []")
 using assms
 proof (induct xs rule: rev_induct)
-  case Nil thus ?case by simp
+  case Nil then show ?case by simp
 next
   case (snoc x xs)
-  hence IH: "[y\<leftarrow>dropWhile ?P xs. key z = key y] = []"
+  then have IH: "[y\<leftarrow>dropWhile ?P xs. key z = key y] = []"
     by (auto simp: sorted_append)
   show ?case
   proof (cases "\<forall>z\<in>set xs. ?P z")
     case True
     show ?thesis
-      using dropWhile_append2[of xs ?P "[x]"] and True by simp
+      using dropWhile_append2 [of xs ?P "[x]"] and True by simp
   next
     case False
     then obtain a where a: "a \<in> set xs" "\<not> ?P a" by auto
     show ?thesis
-      unfolding dropWhile_append1[of a xs ?P, OF a]
+      unfolding dropWhile_append1 [of a xs ?P, OF a]
       using snoc and False by (auto simp: IH sorted_append)
   qed
 qed
 
-lemma filter_by_key_takeWhile[simp]:
+lemma filter_by_key_takeWhile [simp]:
   assumes "sorted (map key xs)"
-  shows "[y\<leftarrow>takeWhile (\<lambda>x. key x \<le> key z) xs. key z = key y]
-    = [y\<leftarrow>xs. key z = key y]"
+  shows "[y\<leftarrow>takeWhile (\<lambda>x. key x \<le> key z) xs. key z = key y] = [y\<leftarrow>xs. key z = key y]"
     (is "[y\<leftarrow>takeWhile ?P xs. key z = key y] = _")
 using assms
 proof (induct xs rule: rev_induct)
-  case Nil thus ?case by simp
+  case Nil then show ?case by simp
 next
   case (snoc x xs)
-  hence IH: "[y\<leftarrow>takeWhile ?P xs. key z = key y] = [y\<leftarrow>xs. key z = key y]"
+  then have IH: "[y\<leftarrow>takeWhile ?P xs. key z = key y] = [y\<leftarrow>xs. key z = key y]"
     by (auto simp: sorted_append)
   show ?case
   proof (cases "\<forall>z\<in>set xs. ?P z")
     case True
     show ?thesis
-      using takeWhile_append2[of xs ?P "[x]"] and True by simp
+      using takeWhile_append2 [of xs ?P "[x]"] and True by simp
   next
     case False
     then obtain a where a: "a \<in> set xs" "\<not> ?P a" by auto
     show ?thesis
-      unfolding takeWhile_append1[of a xs ?P, OF a]
+      unfolding takeWhile_append1 [of a xs ?P, OF a]
       using snoc and False by (auto simp: IH sorted_append)
   qed
 qed
  
-lemma filter_takeWhile_dropWhile_id[simp]:
+lemma filter_takeWhile_dropWhile_id [simp]:
   "filter P (takeWhile Q xs) @ filter P (dropWhile Q xs) = filter P xs"
-  by (simp add: filter_append[symmetric])
+  by (simp flip: filter_append)
 
-lemma filter_by_key_merge_is_append[simp]:
+lemma filter_by_key_merge_is_append [simp]:
   assumes "sorted (map key xs)"
-  shows "[y\<leftarrow>merge key xs ys. key x = key y]
-    = [y\<leftarrow>xs. key x = key y] @ [y\<leftarrow>ys. key x = key y]"
+  shows "[y\<leftarrow>merge key xs ys. key x = key y] =
+    [y\<leftarrow>xs. key x = key y] @ [y\<leftarrow>ys. key x = key y]"
   using assms by (induct xs ys rule: sorted_merge_induct) auto
 
-lemma filter_by_key_merge_pairs[simp]:
+lemma filter_by_key_merge_pairs [simp]:
   assumes "\<forall>xs\<in>set xss. sorted (map key xs)"
-  shows "[y\<leftarrow>concat (merge_pairs key xss). key x = key y]
-    = [y\<leftarrow>concat xss. key x = key y]"
+  shows "[y\<leftarrow>concat (merge_pairs key xss). key x = key y] = [y\<leftarrow>concat xss. key x = key y]"
   using assms by (induct xss rule: merge_pairs.induct) simp_all
 
-lemma filter_by_key_merge_all[simp]:
+lemma filter_by_key_merge_all [simp]:
   assumes "\<forall>xs\<in>set xss. sorted (map key xs)"
-  shows "[y\<leftarrow>merge_all key xss. key x = key y]
-    = [y\<leftarrow>concat xss. key x = key y]"
+  shows "[y\<leftarrow>merge_all key xss. key x = key y] = [y\<leftarrow>concat xss. key x = key y]"
   using assms by (induct xss rule: merge_all.induct) simp_all
 
-lemma filter_by_key_merge_all_sequences[simp]:
-  "[x\<leftarrow>merge_all key (sequences key xs) . key y = key x]
-    = [x\<leftarrow>xs . key y = key x]"
-  using sorted_sequences[of key xs] by simp
+lemma filter_by_key_merge_all_sequences [simp]:
+  "[x\<leftarrow>merge_all key (sequences key xs) . key y = key x] = [x\<leftarrow>xs . key y = key x]"
+  using sorted_sequences [of key xs] by simp
 
 lemma sort_key_merge_all_sequences:
   "sort_key key = merge_all key \<circ> sequences key"
   by (intro ext properties_for_sort_key)
-     (simp_all add: sorted_merge_all[OF sorted_sequences])
+    (simp_all add: sorted_merge_all [OF sorted_sequences])
 
 text \<open>
 Replace existing code equations for @{const sort_key} by
 @{term "merge_all key \<circ> sequences key"}.
 \<close>
-declare sort_key_merge_all_sequences[code]
+declare sort_key_merge_all_sequences [code]
 
 end
 
